SQUASHME Move what can be moved to VerilogSemantics

vera/Verilog/VerilogSemantics.v
@@ -55,6 +55,9 @@ Module RegisterState.
   Definition get_location (st : t) (loc : Location.t) : RawXBV.bit :=
     XBV.bitOf (Location.idx loc) (st (Location.var loc)).
 
+  Definition get_slice {w} (st : t) (slice : Slice.t w) : XBV.xbv w :=
+    XBV.extr (st (Slice.get_var slice)) (Slice.get_lo slice) w.
+
   Definition empty : RegisterState.t := fun var => XBV.exes (Var.varType var).
 
   Lemma empty_get var : empty var = XBV.exes (Var.varType var).
@@ -518,6 +521,16 @@ Module RegisterState.
     rewrite ! set_reg_get_in. reflexivity.
   Qed.
 
+  Lemma match_on_set_reg_same var regs :
+    set_reg var (regs var) regs =( LocationSet.of_variable var )= regs.
+  Proof.
+    intros [v bit_idx] Hloc.
+    apply LocationSet.of_variable_spec in Hloc. cbn in Hloc.
+    destruct Hloc as [Hvar _]. subst v.
+    unfold get_location.
+    rewrite set_reg_get_in. reflexivity.
+  Qed.
+
   Lemma match_on_set_reg_elim_trans C var x regs1 regs2 :
     LocationSet.Disjoint (LocationSet.of_variable var) C ->
     regs1 =( C )= regs2 ->
@@ -570,6 +583,16 @@ Module RegisterState.
     reflexivity.
   Qed.
 
+  Lemma match_on_set_location_same loc wf regs :
+    set_location loc wf (get_location regs loc) regs
+      =( LocationSet.singleton loc )= regs.
+  Proof.
+    intros loc' Hloc'.
+    apply LocationSet.singleton_spec in Hloc'. unfold LocationSet.E.eq in Hloc'. subst loc'.
+    unfold get_location, set_location.
+    rewrite set_reg_get_in, XBV.set_bit_get_in. reflexivity.
+  Qed.
+
   Lemma match_on_set_location_elim2_in C loc wf1 wf2 x regs1 regs2 :
     regs1 =( C )= regs2 ->
     set_location loc wf1 x regs1 =( C )= set_location loc wf2 x regs2.
@@ -612,6 +635,24 @@ Module RegisterState.
       (Slice.get_lo slice + (Location.idx loc - Slice.get_lo slice))%N by lia.
     rewrite ! XBV.set_slice_get_in by lia.
     reflexivity.
+  Qed.
+
+  Lemma match_on_set_slice_same {w} (slice : Slice.t w) regs :
+    set_slice slice (get_slice regs slice) regs
+      =( LocationSet.of_slice slice )= regs.
+  Proof.
+    intros loc Hloc.
+    apply LocationSet.of_slice_spec in Hloc.
+    unfold Slice.has_location in Hloc. destruct Hloc as [Hvar Hidx].
+    unfold get_location, set_slice, get_slice.
+    rewrite <- Hvar, set_reg_get_in.
+    replace (Location.idx loc) with
+      (Slice.get_lo slice + (Location.idx loc - Slice.get_lo slice))%N by lia.
+    rewrite XBV.set_slice_get_in by lia.
+    rewrite XBV.extr_bitOf.
+    - reflexivity.
+    - lia.
+    - apply Slice.wf_width.
   Qed.
 
   Lemma match_on_set_slice_elim2_in {w} C (slice : Slice.t w) x regs1 regs2 :
@@ -1917,6 +1958,15 @@ Hint Rewrite
 Module Facts.
   Import CombinationalOnly.
 
+  Equations read_target {w} (regs : RegisterState.t) (target : Verilog.assign_target w) : XBV.xbv w :=
+    read_target regs (Verilog.AssignVar var) := regs var;
+    read_target regs (Verilog.AssignBit loc _) :=
+      XBV.of_bits [RegisterState.get_location regs loc];
+    read_target regs (Verilog.AssignSlice slice) :=
+      RegisterState.get_slice regs slice;
+    read_target regs (Verilog.AssignConcat lhs rhs) :=
+      XBV.concat (read_target regs lhs) (read_target regs rhs).
+
   Add Parametric Morphism : module_body_reads
     with signature (@Permutation Verilog.module_item) ==> LocationSet.Equal
     as module_body_reads_permute.
@@ -2006,6 +2056,28 @@ Module Facts.
       exact H.
     - rewrite IHtarget1, IHtarget2 by LocationSet.setdec.
       reflexivity.
+  Qed.
+
+  Lemma set_target_from_state {w} (target : Verilog.assign_target w) :
+    Verilog.assign_target_wf target ->
+    forall regs reference,
+      set_target regs target (read_target reference target)
+        =( Verilog.assign_target_writes target )=
+      reference.
+  Proof.
+    intros Hwf.
+    induction Hwf; intros *; simp read_target set_target; simpl.
+    - rewrite RegisterState.match_on_set_reg_elim2.
+      apply RegisterState.match_on_set_reg_same.
+    - rewrite RegisterState.match_on_set_location_elim2 with (wf2:=wf).
+      apply RegisterState.match_on_set_location_same.
+    - rewrite RegisterState.match_on_set_slice_elim2.
+      apply RegisterState.match_on_set_slice_same.
+    - rewrite XBV.extr_concat_high, XBV.extr_concat_low.
+      RegisterState.unpack_match_on.
+      + apply IHHwf1.
+      + rewrite set_target_preserve by assumption.
+        apply IHHwf2.
   Qed.
 
   Lemma set_target_change_regs {w} target value regs1 regs2 :
